@def title = "RealNVP for Physicists"

# RealNVP for physicists
To understand RealNVP, its proper to start from normalizing flow

[https://blog.evjang.com/2018/01/nf1.html](https://blog.evjang.com/2018/01/nf1.html)

## Understand Bijectors

Suppose we have a Bijector $z=f(x)$

**Inference** refers to

$x\sim \hat p_X$

$z=f(x)$

**Generation** referes to

$z\sim p_Z$

$x=f^{-1}(z)$

#### Tractable density

The change of probability

$p_X(x) = p_Z(f(x))\left\vert\det \left(\frac{\partial f(x)}{\partial x^T}\right)\right\vert$
$\log p_X(x) = \log\left(p_Z\left(f(x)\right)\right) + \log\left(\left\vert\det \left(\frac{\partial f(x)}{\partial x^T}\right)\right\vert\right)$

##### The detailed derivation
Let $(a, b) = x$ and $(u, v) = z$

Contributed by Shuo-Hui Li

$$
\iint\limits_{u,v}{p_Z(u,v)}\mathrm{d}{A_Z} = \iint\limits_{a,b}p_X(a,b)\mathrm{d}{A}
$$

$$
\begin{split}
\mathrm{d}{A} &= \mathrm{d}{a}\mathrm{d}{b} \\
&= \left( \frac{\partial{a}}{\partial{u}}\frac{\partial{b}}{\partial{v}}-\frac{\partial{a}}{\partial{v}}\frac{\partial{b}}{\partial{u}}\right) \mathrm{d}{u}\mathrm{d}{v}\\
&=\det{\left\vert\begin{matrix}
\frac{\partial{a}}{\partial{u}} & \frac{\partial{a}}{\partial{v}}\\
\frac{\partial{b}}{\partial{u}} & \frac{\partial{b}}{\partial{v}}
\end{matrix}\right\vert} \mathrm{d}{u}\mathrm{d}{v} \\
\end{split}
$$

Here, the matrix inside the determinant is the Jacobian,
which can be extended to higher dimensions.

$$
\iint\limits_{u,v}{p_Z(u,v)}\mathrm{d}{A_Z} = \iint\limits_{a,b}p_X(a,b)\det{\left\vert\rm Jacobian \right\vert} \mathrm{d}{u}\mathrm{d}{v}
$$

$$
p_Z(u,v) = p_X(a,b)\det{\left\vert\rm Jacobian \right\vert}
$$


#### Example: Box-Muller Algorithm

$z_1, z_2\sim\mathcal U(0,1)$ are two uniform random variables
$$
\begin{cases}
x_1 = \sqrt{-2\ln z_1} \cos(2\pi z_2),\\
x_2 = \sqrt{-2\ln z_1} \sin(2\pi z_2).
\end{cases}
$$
Then, $x_1, x_2$ satisfies  normal distribution.

Try: get the inverse mapping and prove the result.

## RealNVP
A chain of Bijectors, mapping any distribution to normal distribution.
$$
\begin{equation}
H:(u,v)\rightarrow (a,b) \\
\left\{
\begin{array}{rl}
a &= m^0(u,v)u+m^1(u,v)\\
b &=m^2(u,v)v+m^3(u,v)\\
\end{array}
\right.
\end{equation}
$$
