@def title = "Solving random walk on graphs with tails"

# Solving random walk on graphs with tails

## References

1. [Quantum scattering theory on graphs with tails](https://arxiv.org/abs/0906.2825) (Martin Varbanov, Todd A. Brun, 2009)

## Half chain
Let the hamiltonian of a half chain be
$$H_{1/2} = \frac{1}{2}  \sum_{n=0}^\infty |n\rangle\langle {n+1}| + h.c.$$

The eigenvalues and eigenvectors of a full chain are $\cos(k)$ and $| k\rangle = e^{ikn} |n\rangle$ respectively.
Given an eigenvector of a full chain, the effect of applying the half chain Hamiltonian on it is
$$
\begin{align*}\label{eq:chain}
H_{1/2} |k\rangle_{1/2} &= \sum_{n=0}^{\infty}\frac{1}{2}e^{ikn}(|n-1\rangle + |n+1\rangle)\\
&= \sum_{n=0}^{\infty}\left(\frac{1}{2}(e^{ik(n-1)}+e^{ik(n+1)})|n\rangle\right) - \frac{1}{2}e^{-ik}|0\rangle\\
&=\cos(k) |k\rangle_{1/2} - \frac{1}{2}e^{-ik}|0\rangle
\end{align*}
$$
where $|k\rangle_{1/2} = \sum_{n=0}^{\infty} |n\rangle\langle n|k\rangle$.


## Graphs with tails

Let $G=(V,E)$ be a graph with some of its vertices $V'\subseteq V$ attached to half chains (or tails) and each vertex can be attached to at most one tail. The model Hamiltonian is

$$
H = H_G + \sum_{v\in V'} H_v
$$

where $H_v = \frac{1}{2}  \sum_{n=0}^\infty |n_v\rangle\langle {n+1}_v| + h.c.$ is a 1D chain model and $H_G$ is the Hamiltonian on a graph.
In the following, unless specified explicitly, $\sum_v$ stands for $\sum_{v\in V'}$.
Let us decompose the wave function on the graph into three parts.
![](/assets/plot/halfchain.png)

$$
\begin{equation*}\label{eq:threeparts}
|\psi\rangle = |\psi_G\rangle + \sum_v |\psi_v\rangle - \sum_v a_v|0_v\rangle
\end{equation*}
$$
where $|\psi_G\rangle = \sum_{v\in V}|v\rangle\langle v|\psi\rangle$ (note in our definition, $|v\rangle = |0_v\rangle$), $|\psi_v\rangle = \sum_{n=0}^\infty|n_v\rangle\langle n_v|\psi\rangle$ and $a_v = \langle 0_v|\psi_G\rangle = \langle 0_v|\psi\rangle_v$.

To solve the eigen-decomposition problem $H |\psi\rangle = E|\psi\rangle$, we have
$$
\begin{align*}\label{eq:hpsi}
H |\psi\rangle &= H_G |\psi_G\rangle \textcolor{lightgray}{+ H_G\sum_v(|\psi_v\rangle - a_v|0_v\rangle)}\\
&\textcolor{lightgray}{+\sum_v H_v (|\psi_G\rangle - \sum_{v'} a_{v'}|0_{v'}\rangle)} + \sum_v H_v|\psi_v\rangle
\end{align*}
$$
where gray parts are zeroed out.

### Propagating states
Let us **assume** $|\psi_v\rangle = I_v|-k\rangle + R_v|k\rangle$, we have
$$a_v = I_v+R_v. \label{eq:av}$$
By inserting \eqref{eq:chain} to \eqref{eq:hpsi}, we have
$$\label{eq:hpsiprop}
H |\psi\rangle = H_G |\psi_G\rangle + \sum_v \cos(k)|\psi_v\rangle - \left(\frac{I_v}{2}e^{ik} + \frac{R_v}{2}e^{-ik}\right)|0_v\rangle
$$
For this ansatz, the eigenvalue of $H$ has to be $E=\cos(k)$. By using \eqref{eq:threeparts} and \eqref{eq:av}
$$
\begin{align*}
&\cos(k) \left(|\psi_G\rangle \textcolor{lightgray}{+ \sum_v |\psi_v\rangle} - \sum_v (I_v + R_v)|0_v\rangle\right) \\
= &H_G |\psi_G\rangle \textcolor{lightgray}{+ \sum_v \cos(k)|\psi_v\rangle} - \sum_v\left(\frac{I_v}{2}e^{ik} + \frac{R_v}{2}e^{-ik}\right)|0_v\rangle
\end{align*}
$$

That is
$$
\begin{align*}
H_G|\psi_G\rangle = &\cos(k) |\psi\rangle_G+ \sum_{v}\left(-\cos(k)(I_v + R_v) +\frac{I_v}{2}e^{ik} + \frac{R_v}{2}e^{-ik}\right)|0_v\rangle\\
= &\cos(k) |\psi\rangle_G- \sum_{v}\left(\frac{I_v}{2}e^{-ik} + \frac{R_v}{2}e^{ik}\right)|0_v\rangle
\end{align*}
$$

Let us **assume** the scattering is from vertex $w$, i.e. $I_w = 1$ and $I_{v\neq w} = 0$.
We have
$$\label{eq:standardform}
\begin{align*}
H_G|\psi_G\rangle = &\cos(k) |\psi\rangle_G-\frac{1}{2}e^{-ik}|0_w\rangle - \sum_{v}\frac{R_v}{2}e^{ik}|0_v\rangle
\end{align*}
$$


#### Key point: Equation \eqref{eq:standardform} is a quadratic linear equation
Let $z = e^{ik}$, we have
$$\label{eq:standardform}
\begin{align*}
&2H_G z|\psi_G\rangle = (1+z^2) |\psi\rangle_G-|0_w\rangle - \sum_{v}R_vz^2|0_v\rangle\\
&(1 - 2H_G z|\psi_G\rangle + Q z^2)|\psi\rangle_G = (1-z^2)|0_w\rangle
\end{align*}
$$

where
$$
Q = 1 - \sum_v| 0_v\rangle\langle 0_v |
$$
since 
$$
a_v = \langle 0_v|\psi\rangle_G = \begin{cases}
R_v &, v \neq w\\
1+R_w &, v = w
\end{cases}
$$

Except the $-2$ before $H_G$ due to the difference in convension, \eqref{eq:standardform} is the same as Eq. 12 in Ref. 1.

### Bound states
There are two types of bound states. The first type with $|\psi\rangle_v = 0$ is trivial.
In the following, we discuss the second type: $k = i\kappa$ is pure imaginary.
Let us **assume** $$\label{eq:psibound}|\psi_v\rangle = a_v|\kappa\rangle$$ with $|\kappa\rangle = e^{-\kappa n_v} |n_v\rangle$.
Following the same derivation from \eqref{eq:hpsiprop} to \eqref{eq:standardform}, we have
$$
H |\psi\rangle = H_G |\psi_G\rangle + \sum_v \cosh(\kappa)|\psi_v\rangle - \frac{a_v}{2}e^{\kappa}|0_v\rangle
$$
For this ansatz, the eigenvalue of $H$ has to be $E=\cosh(\kappa)$. By using \eqref{eq:threeparts} and \eqref{eq:psibound}
$$
\begin{align*}
&\cosh(\kappa) \left(|\psi_G\rangle \textcolor{lightgray}{+ \sum_v |\psi_v\rangle} - \sum_v a_v|0_v\rangle\right) \\
= &H_G |\psi_G\rangle \textcolor{lightgray}{+ \sum_v \cosh(\kappa)|\psi_v\rangle} - \sum_v\frac{a_v}{2}e^{\kappa}|0_v\rangle,\\
&H_G|\psi_G\rangle = \cosh(\kappa) |\psi\rangle_G - \sum_{v}\frac{a_v}{2}e^{-\kappa}|0_v\rangle\\
\end{align*}
$$

Let $z_b = e^{-\kappa}$, we have a new quadratic linear equation for the bounded states

$$\label{eq:standardformb}
(1-2H_Gz_b+Qz_b^2)|\psi_G\rangle = 0
$$

